Source/DafnyTestGeneration/RequireBasedModifier.cs
@@ -10,33 +10,24 @@ namespace DafnyTestGeneration {
   /// </summary>
   public class RequireBasedModifier : ProgramModifier {
     private Program? program; // the original program
-    private List<RequirePartitionFromProc> partitions = new();
-    private List<RequirePartitionFromImpl> partitionsImpls = new();
+    private List<InputPartition> partitions = new();
+    private List<Procedure> procsWithCall = new();
+    private List<Procedure> procs = new();
     private List<Implementation> impls = new();
 
     protected override IEnumerable<ProgramModification> GetModifications(Program p) {
-      partitions = new List<RequirePartitionFromProc>();
       var result = new List<ProgramModification>();
-
-      partitionsImpls = new List<RequirePartitionFromImpl>();
 
       // populate partitions
       p = VisitProgram(p);
 
-      /*foreach (var partition in partitions) {
-        if (partition.HasUserDefinedPreconditions())
-          result.Add(new ProgramModification(p, ProcedureName ?? partition.procedure.Name));
-      }*/
-
       Console.Error.WriteLine("\n======== Extraction of Modifications ==========\n");
-      foreach (var partition in partitionsImpls) {
+      foreach (var partition in partitions) {
         Console.Error.WriteLine("Partition");
-        partition.ExtractUserDefinedPreconditions();
         Console.Error.WriteLine("\t Has user defined preconditions?");
         if (partition.HasUserDefinedPreconditions()) {
           Console.Error.WriteLine("\t yes - generating modifications");
           result.AddRange(partition.GetProgramModifications(p, impls));
-          //result.Add(new ProgramModification(p, ProcedureName ?? partition.impl.Proc.Name));
         }
       }
 
@@ -53,19 +44,19 @@ namespace DafnyTestGeneration {
         return base.VisitProcedure(node);
       }
 
-      /*if (node.Name.StartsWith("Impl$$"))
-        partitions.Add(new RequirePartitionFromProc(node));
-      */
+      if (node.Name.StartsWith("Impl$$")) {
+        partitions.Add(new InputPartition(node, procsWithCall));
+        procs.Add(node);
+      }
+      if (node.Name.StartsWith("Call$$")) {
+        procsWithCall.Add(node);
+      }
       return base.VisitProcedure(node);
     }
 
     public override Implementation VisitImplementation(Implementation node) {
       Console.Error.WriteLine("visit impl: " + node.Name);
-      if (node.Name.StartsWith("CheckWellformed$$")) {
-        Console.Error.WriteLine("\tAdded to assume parsing list");
-        partitionsImpls.Add(new RequirePartitionFromImpl(node));
-      } else if (node.Name.StartsWith("Impl$$")) {
-        Console.Error.WriteLine("\tAdded to impl injection list");
+      if (node.Name.StartsWith("Impl$$")) {
         impls.Add(node);
       }
 
@@ -78,135 +69,110 @@ namespace DafnyTestGeneration {
     }
 
 
-    private class RequirePartitionFromProc {
+    private class InputPartition {
       public readonly Procedure procedure;
 
-      internal RequirePartitionFromProc(Procedure proc) {
+      public readonly List<Procedure> proceduresWithCall;
+      public List<Requires> requires;
+      internal InputPartition(Procedure proc, List<Procedure> withCalls) {
         procedure = proc;
-      }
+        this.proceduresWithCall = withCalls;
+        this.requires = new();
 
-      internal bool HasUserDefinedPreconditions() {
-        List<Requires> req = procedure.Requires;
-        Console.Error.WriteLine("Procedure: " + procedure.Name);
-        foreach (var r in req) {
-          Console.Error.WriteLine("\tRequire: " + r.Comment + " - " + r.Condition);
-        }
-        return false;
-      }
 
-    }
-
-    private class RequirePartitionFromImpl {
-      public readonly Implementation impl;
-
-      public Block AssumeBlock;
-
-      public readonly List<AssumeCmd> requireAssumes;
-
-      internal RequirePartitionFromImpl(Implementation imp) {
-        impl = imp;
-        requireAssumes = new();
-      }
-
-      internal void ExtractUserDefinedPreconditions() {
-        // A hack to make sure the Implementation is for a real implementation, rather than
-        // a function called in the specification
-        String AddMethodComment = "AddMethodImpl:";
-        bool HasSeenAddMethodComment = false;
-
-        StmtList req = impl.StructuredStmts;
-        List<Block> blocks = impl.Blocks;
-        Console.Error.WriteLine("Impl: " + impl);
-        foreach (var block in blocks) {
-          Console.Error.WriteLine("\t" + block.Label);
-          List<Cmd> cmds = block.cmds;
-          foreach (var cmd in cmds) {
-            // we have seen the necessary comment
-            if (HasSeenAddMethodComment) {
-              // Add Assumes
-              if (cmd is AssumeCmd assume) {
-                Console.Error.WriteLine("******* ADD ASSUME BELOW");
-                requireAssumes.Add(assume);
-              }
-
-              // Havoc stops
-              if (cmd is HavocCmd havoc) {
-                // remove the capture state
-                requireAssumes.RemoveAt(0);
-                Console.Error.WriteLine("******* TERMINATING HAVOC BELOW");
-                return;
-              }
-            }
-
-            // search for the comment key to know its a real implementation
-            if (cmd is CommentCmd commentLine) {
-              if (commentLine.Comment.StartsWith(AddMethodComment)) {
-                HasSeenAddMethodComment = true;
-                AssumeBlock = block;
-                Console.Error.WriteLine("******* FOUND COMMENT BELOW");
-              }
-            }
-            Console.Error.Write("\t\t" + cmd);
+        Console.Error.WriteLine("Found Procedure: " + procedure.Name);
+        bool foundComment = false;
+        foreach (var r in procedure.Requires) {
+          Console.Error.WriteLine("\tWith Require: " + r.Comment + " - " + r.Condition);
+          if (!foundComment &&
+              r.Comment != null &&
+              r.Comment.StartsWith("user-defined preconditions")) {
+            foundComment = true;
+          }
+          if (foundComment) {
+            Console.Error.WriteLine("\t\tkept require ^^");
+            this.requires.Add(r);
           }
         }
       }
 
+      internal bool HasUserDefinedPreconditions() {
+        return this.requires.Count > 0;
+      }
 
-      // Program p will be modified
-      // The implementation list allows us to insert into the original program's 
-      // implementation rather than the well-formed
       internal List<ProgramModification> GetProgramModifications(Program p, List<Implementation> impls) {
-        List<ProgramModification> mods = new();
+        String matchingPartialName = procedure.Name.Substring(4);
 
-        Console.Error.WriteLine("Get Program Modifications: ");
-        // for each assume, generate positive and negative assert modification
-        foreach (AssumeCmd assume in requireAssumes) {
-          Console.Error.WriteLine("Statement:" + assume.ToString());
-          String text = assume.ToString().Replace("assume ", "assert (").Replace(";\n", ") == false;\n");
-          Console.Error.WriteLine("Replaced With:" + text);
-
-          //positive
-          Cmd positiveCommand = GetCmd(text);
-          Console.Error.WriteLine("Command: " + positiveCommand);
-
-          // negative
-          // TODO: 
-
-          String methodName = impl.Name.Replace("CheckWellformed$$", "");
-          // find matching impl
-          Implementation i = impls.Find(x => x.Name.EndsWith(methodName));
-          if (i == null) {
-            Console.Error.WriteLine("******************UNEXPECTED TERMINATION*************************");
-            Console.Error.WriteLine("******************UNEXPECTED TERMINATION*************************");
-            Console.Error.WriteLine("******************UNEXPECTED TERMINATION*************************");
-            Console.Error.WriteLine("******************UNEXPECTED TERMINATION*************************");
-          } else {
-            // Add to the implementation
-            Block firstBlock = i.Blocks[0];
-            Console.Error.WriteLine("Injected into the Implementation hopefully");
-            firstBlock.cmds.Insert(0, positiveCommand);
-            mods.Add(new ProgramModification(p, impl.Name));
-            firstBlock.cmds.RemoveAt(0);
-
-            // Also lets add to the checkwellformed
-            AssumeBlock.cmds.Insert(0, positiveCommand);
-            mods.Add(new ProgramModification(p, impl.Name));
-            AssumeBlock.cmds.RemoveAt(0);
+        // strip out requires statements everywhere.
+        Procedure call = this.proceduresWithCall.Find(x => x.Name.EndsWith(matchingPartialName));
+        Console.Error.WriteLine("Found matching call" + call);
+        /*foreach (var r in this.requires) {
+          procedure.Requires.Remove(r); // remove the user defined requires (except we do want to only comment out one at a time later)
+          // also need to remove it from the `procedure Call$$` requires as well?
+          if (call != null) {
+            Requires matchingRequires = call.Requires.Find(x => x.Condition.ToString().Equals(r.Condition.ToString()));
+            call.Requires.Remove(matchingRequires);
           }
+        }*/
+
+        List<ProgramModification> mods = new();
+        Implementation matchingImpl = impls.Find(x => x.Name.EndsWith(matchingPartialName));
+        Requires firstRequires = requires[0];
+        if (matchingImpl != null) {
+          Console.Error.WriteLine("Input Partition with matching Partial Name (" + matchingPartialName + ") = " + matchingImpl.Name);
+          // inject the assert statements
+          var firstBlock = matchingImpl.Blocks[0];
+          if (firstBlock != null) {
 
 
-          //AssumeBlock.cmds.Insert(0, positiveCommand);
-          //mods.Add(new ProgramModification(p, impl.Name));
-          //AssumeBlock.cmds.RemoveAt(0);
+            // new stuff for each requires
+            foreach (Requires aRequire in requires) {
+              // strip out require statements, to be added back in later
+              procedure.Requires.Remove(aRequire);
+              Requires matchingRequires = null;
+              if (call != null) {
+                matchingRequires = call.Requires.Find(x => x.Condition.ToString().Equals(aRequire.Condition.ToString()));
+                call.Requires.Remove(matchingRequires);
+              }
 
 
 
+
+              String negatedRequires = "assert (" + aRequire.Condition.ToString() + ") == Lit(false);";
+              String falseAssertion = "assert false;";
+              Console.Error.WriteLine("Injecting:" + negatedRequires);
+              Console.Error.WriteLine("Injecting:" + falseAssertion);
+
+              //positive
+              Cmd assumeTrueFirst = GetAssumeCmd(new List<string>());
+              Cmd negatedRequiresCmd = GetCmd(negatedRequires);
+              Cmd assumeTrueSecond = GetAssumeCmd(new List<string>());
+              Cmd falseAssertionCmd = GetCmd(falseAssertion);
+              Console.Error.WriteLine("Command: " + negatedRequiresCmd);
+              Console.Error.WriteLine("Command: " + falseAssertionCmd);
+
+              firstBlock.cmds.Insert(6, assumeTrueFirst);
+              firstBlock.cmds.Insert(7, negatedRequiresCmd);
+              firstBlock.cmds.Insert(8, assumeTrueSecond);
+              firstBlock.cmds.Insert(9, falseAssertionCmd);
+              mods.Add(new ProgramModification(p, procedure.Name));
+              firstBlock.cmds.RemoveAt(9);
+              firstBlock.cmds.RemoveAt(8);
+              firstBlock.cmds.RemoveAt(7);
+              firstBlock.cmds.RemoveAt(6);
+
+
+              // add the stripped out require statements
+              procedure.Requires.Add(aRequire);
+              if (call != null && matchingRequires != null) {
+                call.Requires.Add(matchingRequires);
+              }
+
+            }
+          }
         }
-        return mods;
-      }
 
-      internal bool HasUserDefinedPreconditions() {
-        return requireAssumes.Count > 0;
+        return mods;
       }
 
     }
