string_project/str_recurse_test-java/str__recurseUnitTests_Compile/__default.java
@@ -3,61 +3,18 @@
 package str__recurseUnitTests_Compile;
 
 import M_Compile.*;
-import java.lang.reflect.*;
 
-@SuppressWarnings({ "unchecked", "deprecation" })
+@SuppressWarnings({"unchecked", "deprecation"})
 public class __default {
-  public static void main(String[] args) throws Exception {
-    for (Method method : __default.class.getDeclaredMethods()) {
-      if (!method.getName().startsWith("test"))
-        continue;
-      Object result = method.invoke(null, mockParameters(method));
-      String resultString = result == null ? "null" : result.toString();
-      System.out.println(method.getName() + " " + resultString);
-    }
-  }
-
-  public static Object[] mockParameters(Method method) {
-    Object[] parameters = null;
-    try {
-      Class<?>[] types = method.getParameterTypes();
-      parameters = new Object[types.length];
-      for (int i = 0; i < types.length; i++)
-        parameters[i] = types[i].getConstructor().newInstance();
-    } catch (Exception e) {
-      e.printStackTrace();
-    }
-    return parameters;
-  }
   public __default() {
   }
-  public static dafny.DafnySequence<? extends Character> test0()
+  public static java.math.BigInteger test0()
   {
-    dafny.DafnySequence<? extends Character> r0 = dafny.DafnySequence.<Character> empty(dafny.TypeDescriptor.CHAR);
+    java.math.BigInteger r0 = java.math.BigInteger.ZERO;
     if(true) {
-      dafny.DafnySequence<? extends Character> _out2;
-      _out2 = M_Compile.__default.replaceRecursive(dafny.DafnySequence.of('!', 'a'), dafny.DafnySequence.of('"', 'a'), dafny.DafnySequence.of('a'));
-      r0 = _out2;
-    }
-    return r0;
-  }
-  public static dafny.DafnySequence<? extends Character> test1()
-  {
-    dafny.DafnySequence<? extends Character> r0 = dafny.DafnySequence.<Character> empty(dafny.TypeDescriptor.CHAR);
-    if(true) {
-      dafny.DafnySequence<? extends Character> _out3;
-      _out3 = M_Compile.__default.replaceRecursive(dafny.DafnySequence.of('a', 'a', 'a'), dafny.DafnySequence.of('a', 'a'), dafny.DafnySequence.of('a'));
-      r0 = _out3;
-    }
-    return r0;
-  }
-  public static dafny.DafnySequence<? extends Character> test2()
-  {
-    dafny.DafnySequence<? extends Character> r0 = dafny.DafnySequence.<Character> empty(dafny.TypeDescriptor.CHAR);
-    if(true) {
-      dafny.DafnySequence<? extends Character> _out4;
-      _out4 = M_Compile.__default.replaceRecursive(dafny.DafnySequence.of('a'), dafny.DafnySequence.of('a', 'a'), dafny.DafnySequence.of('a'));
-      r0 = _out4;
+      java.math.BigInteger _out0 = java.math.BigInteger.ZERO;
+      _out0 = M_Compile.__default.foo(java.math.BigInteger.valueOf(11L), java.math.BigInteger.valueOf(6L));
+      r0 = _out0;
     }
     return r0;
   }
