string_project/str_recurse_test.dfy
@@ -1,4 +1,13 @@
 include "/workspaces/dafny/string_project/str_recurse.dfy"
 module str_recurseUnitTests {
 import M
+method test0() returns (r0:int)  {
+r0 := M.foo(11, 6);
+}
+method test1() returns (r0:int)  {
+r0 := M.foo(11, 5);
+}
+method test3() returns (r0:int)  {
+r0 := M.foo(10, 6);
+}
 }
