string_project/str_recurse_boogie_modification_1_preexe_RES.bpl
@@ -1,0 +1,2160 @@
+<no file>(1498,4): Error: This assertion might not hold.
+Execution trace:
+    (1609,3): anon0
+Augmented execution trace:
+Impl | Impl$$M.__default.foo | 11 | 6
+Types | int | int
+
+*** MODEL
+#_System._tuple#0._#Make0 -> T@U!val!63
+##_System._tuple#0._#Make0 -> T@U!val!40
+##_System._tuple#2._#Make2 -> T@U!val!37
+$_Frame -> 
+$_Frame@0 -> T@U!val!66
+$_reverifyPost -> 
+$$Language$Dafny -> true
+$FunctionContextHeight -> 0
+$Heap -> T@U!val!65
+$OneHeap -> T@U!val!58
+$Tick -> 
+a#0 -> 11
+alloc -> T@U!val!22
+allocName -> T@U!val!23
+b#0 -> 6
+boolType -> T@T!val!2
+BoxType -> T@T!val!13
+c#0 -> 
+charType -> T@T!val!14
+class._System.array? -> T@U!val!28
+class._System.bool -> T@U!val!18
+class._System.int -> T@U!val!17
+class._System.multiset -> T@U!val!21
+class._System.object? -> T@U!val!25
+class._System.seq -> T@U!val!20
+class._System.set -> T@U!val!19
+class._System.Tuple0 -> T@U!val!42
+class._System.Tuple2 -> T@U!val!39
+class.M.__default -> T@U!val!43
+ClassNameType -> T@T!val!8
+DatatypeTypeType -> T@T!val!17
+defass#c#0 -> 
+DtCtorIdType -> T@T!val!11
+HandleTypeType -> T@T!val!20
+intType -> T@T!val!0
+LayerTypeType -> T@T!val!18
+MapType1Type -> T@T!val!15
+NameFamilyType -> T@T!val!10
+null -> T@U!val!60
+realType -> T@T!val!1
+refType -> T@T!val!16
+regexType -> T@T!val!5
+rmodeType -> T@T!val!3
+stringType -> T@T!val!4
+TagBool -> T@U!val!5
+TagChar -> T@U!val!6
+TagClass -> T@U!val!16
+Tagclass._System.___hFunc0 -> T@U!val!34
+Tagclass._System.___hFunc1 -> T@U!val!31
+Tagclass._System.___hPartialFunc0 -> T@U!val!35
+Tagclass._System.___hPartialFunc1 -> T@U!val!32
+Tagclass._System.___hTotalFunc0 -> T@U!val!36
+Tagclass._System.___hTotalFunc1 -> T@U!val!33
+Tagclass._System.array -> T@U!val!30
+Tagclass._System.array? -> T@U!val!29
+Tagclass._System.nat -> T@U!val!24
+Tagclass._System.object -> T@U!val!27
+Tagclass._System.object? -> T@U!val!26
+Tagclass._System.Tuple0 -> T@U!val!41
+Tagclass._System.Tuple2 -> T@U!val!38
+Tagclass.M.__default -> T@U!val!44
+TagIMap -> T@U!val!15
+TagInt -> T@U!val!7
+TagISet -> T@U!val!11
+TagMap -> T@U!val!14
+TagMultiSet -> T@U!val!12
+TagORDINAL -> T@U!val!9
+TagReal -> T@U!val!8
+TagSeq -> T@U!val!13
+TagSet -> T@U!val!10
+TBool -> T@U!val!0
+TChar -> T@U!val!1
+Tclass._System.nat -> T@U!val!59
+Tclass._System.object -> T@U!val!61
+Tclass._System.object? -> T@U!val!57
+Tclass._System.Tuple0 -> T@U!val!62
+Tclass.M.__default -> T@U!val!64
+TInt -> T@U!val!2
+TORDINAL -> T@U!val!4
+TReal -> T@U!val!3
+tytagFamily$_#Func0 -> T@U!val!51
+tytagFamily$_#Func1 -> T@U!val!48
+tytagFamily$_#PartialFunc0 -> T@U!val!52
+tytagFamily$_#PartialFunc1 -> T@U!val!49
+tytagFamily$_#TotalFunc0 -> T@U!val!53
+tytagFamily$_#TotalFunc1 -> T@U!val!50
+tytagFamily$_default -> T@U!val!56
+tytagFamily$_tuple#0 -> T@U!val!55
+tytagFamily$_tuple#2 -> T@U!val!54
+tytagFamily$array -> T@U!val!47
+tytagFamily$nat -> T@U!val!45
+tytagFamily$object -> T@U!val!46
+TyTagFamilyType -> T@T!val!12
+TyTagType -> T@T!val!7
+TyType -> T@T!val!6
+unique-value!100 -> distinct-elems!84!val!14
+unique-value!101 -> distinct-elems!84!val!15
+unique-value!102 -> distinct-elems!84!val!16
+unique-value!103 -> distinct-elems!84!val!17
+unique-value!104 -> distinct-elems!84!val!18
+unique-value!105 -> distinct-elems!84!val!19
+unique-value!106 -> distinct-elems!84!val!20
+unique-value!107 -> distinct-elems!84!val!21
+unique-value!108 -> distinct-elems!84!val!22
+unique-value!109 -> distinct-elems!84!val!23
+unique-value!110 -> distinct-elems!84!val!24
+unique-value!111 -> distinct-elems!84!val!25
+unique-value!112 -> distinct-elems!84!val!26
+unique-value!113 -> distinct-elems!84!val!27
+unique-value!114 -> distinct-elems!84!val!28
+unique-value!115 -> distinct-elems!84!val!29
+unique-value!116 -> distinct-elems!84!val!30
+unique-value!117 -> distinct-elems!84!val!31
+unique-value!118 -> distinct-elems!84!val!32
+unique-value!119 -> distinct-elems!84!val!33
+unique-value!120 -> distinct-elems!84!val!34
+unique-value!121 -> distinct-elems!84!val!35
+unique-value!122 -> distinct-elems!84!val!36
+unique-value!123 -> distinct-elems!84!val!37
+unique-value!124 -> distinct-elems!84!val!38
+unique-value!125 -> distinct-elems!84!val!39
+unique-value!126 -> distinct-elems!84!val!40
+unique-value!127 -> distinct-elems!84!val!41
+unique-value!128 -> distinct-elems!84!val!42
+unique-value!129 -> distinct-elems!84!val!43
+unique-value!130 -> distinct-elems!84!val!44
+unique-value!131 -> distinct-elems!84!val!45
+unique-value!132 -> distinct-elems!84!val!46
+unique-value!133 -> distinct-elems!84!val!47
+unique-value!134 -> distinct-elems!84!val!48
+unique-value!135 -> distinct-elems!84!val!49
+unique-value!136 -> distinct-elems!84!val!50
+unique-value!137 -> distinct-elems!84!val!51
+unique-value!138 -> distinct-elems!84!val!52
+unique-value!139 -> distinct-elems!84!val!53
+unique-value!140 -> distinct-elems!84!val!54
+unique-value!141 -> distinct-elems!84!val!55
+unique-value!142 -> distinct-elems!84!val!56
+unique-value!86 -> distinct-elems!84!val!0
+unique-value!87 -> distinct-elems!84!val!1
+unique-value!88 -> distinct-elems!84!val!2
+unique-value!89 -> distinct-elems!84!val!3
+unique-value!90 -> distinct-elems!84!val!4
+unique-value!91 -> distinct-elems!84!val!5
+unique-value!92 -> distinct-elems!84!val!6
+unique-value!93 -> distinct-elems!84!val!7
+unique-value!94 -> distinct-elems!84!val!8
+unique-value!95 -> distinct-elems!84!val!9
+unique-value!96 -> distinct-elems!84!val!10
+unique-value!97 -> distinct-elems!84!val!11
+unique-value!98 -> distinct-elems!84!val!12
+unique-value!99 -> distinct-elems!84!val!13
+_System.array.Length -> {
+  else -> 0
+}
+_System.Tuple0.___hMake0_q -> {
+  else -> false
+}
+_System.Tuple0#Equal -> {
+  else -> false
+}
+_System.Tuple2.___hMake2_q -> {
+  else -> false
+}
+_System.Tuple2._0 -> {
+  else -> T@U!val!0
+}
+_System.Tuple2._1 -> {
+  else -> T@U!val!0
+}
+_System.Tuple2#Equal -> {
+  else -> false
+}
+#_System._tuple#2._#Make2 -> {
+  else -> T@U!val!0
+}
+$Box -> {
+  else -> T@U!val!0
+}
+$HeapSucc -> {
+  else -> false
+}
+$HeapSuccGhost -> {
+  else -> false
+}
+$Is -> {
+  T@U!val!63 T@U!val!62 -> true
+  else -> true
+}
+$IsA#_System.Tuple0 -> {
+  else -> false
+}
+$IsA#_System.Tuple2 -> {
+  else -> false
+}
+$IsAlloc -> {
+  else -> false
+}
+$IsAllocBox -> {
+  else -> false
+}
+$IsBox -> {
+  else -> false
+}
+$IsGhostField -> {
+  T@U!val!22 -> false
+  else -> false
+}
+$IsGoodHeap -> {
+  T@U!val!58 -> true
+  T@U!val!65 -> true
+  else -> true
+}
+$IsGoodMultiSet -> {
+  else -> false
+}
+$IsHeapAnchor -> {
+  T@U!val!65 -> true
+  else -> true
+}
+$LS -> {
+  else -> T@U!val!0
+}
+$Unbox -> {
+  else -> T@U!val!0
+}
+Add -> {
+  else -> 0
+}
+Apply0 -> {
+  else -> T@U!val!0
+}
+Apply1 -> {
+  else -> T@U!val!0
+}
+AtLayer -> {
+  else -> T@U!val!0
+}
+bool_2_U -> {
+  false -> false
+  else -> false
+}
+BoxRank -> {
+  else -> 0
+}
+char#FromInt -> {
+  else -> T@U!val!0
+}
+char#Minus -> {
+  else -> T@U!val!0
+}
+char#Plus -> {
+  else -> T@U!val!0
+}
+char#ToInt -> {
+  else -> 0
+}
+ControlFlow -> {
+  0 0 -> 63373
+  0 54326 -> (- 63445)
+  0 63373 -> 54326
+  else -> 63373
+}
+Ctor -> {
+  T@T!val!0 -> 0
+  T@T!val!1 -> 1
+  T@T!val!10 -> 10
+  T@T!val!11 -> 11
+  T@T!val!12 -> 12
+  T@T!val!13 -> 13
+  T@T!val!14 -> 14
+  T@T!val!15 -> 19
+  T@T!val!16 -> 20
+  T@T!val!17 -> 21
+  T@T!val!18 -> 22
+  T@T!val!19 -> 15
+  T@T!val!2 -> 2
+  T@T!val!20 -> 23
+  T@T!val!21 -> 25
+  T@T!val!3 -> 3
+  T@T!val!4 -> 4
+  T@T!val!5 -> 5
+  T@T!val!6 -> 6
+  T@T!val!7 -> 7
+  T@T!val!8 -> 8
+  T@T!val!9 -> 9
+  else -> 0
+}
+DatatypeCtorId -> {
+  T@U!val!63 -> T@U!val!40
+  else -> T@U!val!40
+}
+DeclName -> {
+  T@U!val!22 -> T@U!val!23
+  else -> T@U!val!23
+}
+DeclType -> {
+  else -> T@U!val!0
+}
+distinct-aux-f!!85 -> {
+  T@U!val!0 -> distinct-elems!84!val!0
+  T@U!val!1 -> distinct-elems!84!val!1
+  T@U!val!10 -> distinct-elems!84!val!10
+  T@U!val!11 -> distinct-elems!84!val!11
+  T@U!val!12 -> distinct-elems!84!val!12
+  T@U!val!13 -> distinct-elems!84!val!13
+  T@U!val!14 -> distinct-elems!84!val!14
+  T@U!val!15 -> distinct-elems!84!val!15
+  T@U!val!16 -> distinct-elems!84!val!16
+  T@U!val!17 -> distinct-elems!84!val!17
+  T@U!val!18 -> distinct-elems!84!val!18
+  T@U!val!19 -> distinct-elems!84!val!19
+  T@U!val!2 -> distinct-elems!84!val!2
+  T@U!val!20 -> distinct-elems!84!val!20
+  T@U!val!21 -> distinct-elems!84!val!21
+  T@U!val!22 -> distinct-elems!84!val!22
+  T@U!val!23 -> distinct-elems!84!val!23
+  T@U!val!24 -> distinct-elems!84!val!24
+  T@U!val!25 -> distinct-elems!84!val!25
+  T@U!val!26 -> distinct-elems!84!val!26
+  T@U!val!27 -> distinct-elems!84!val!27
+  T@U!val!28 -> distinct-elems!84!val!28
+  T@U!val!29 -> distinct-elems!84!val!29
+  T@U!val!3 -> distinct-elems!84!val!3
+  T@U!val!30 -> distinct-elems!84!val!30
+  T@U!val!31 -> distinct-elems!84!val!31
+  T@U!val!32 -> distinct-elems!84!val!32
+  T@U!val!33 -> distinct-elems!84!val!33
+  T@U!val!34 -> distinct-elems!84!val!34
+  T@U!val!35 -> distinct-elems!84!val!35
+  T@U!val!36 -> distinct-elems!84!val!36
+  T@U!val!37 -> distinct-elems!84!val!37
+  T@U!val!38 -> distinct-elems!84!val!38
+  T@U!val!39 -> distinct-elems!84!val!39
+  T@U!val!4 -> distinct-elems!84!val!4
+  T@U!val!40 -> distinct-elems!84!val!40
+  T@U!val!41 -> distinct-elems!84!val!41
+  T@U!val!42 -> distinct-elems!84!val!42
+  T@U!val!43 -> distinct-elems!84!val!43
+  T@U!val!44 -> distinct-elems!84!val!44
+  T@U!val!45 -> distinct-elems!84!val!45
+  T@U!val!46 -> distinct-elems!84!val!46
+  T@U!val!47 -> distinct-elems!84!val!47
+  T@U!val!48 -> distinct-elems!84!val!48
+  T@U!val!49 -> distinct-elems!84!val!49
+  T@U!val!5 -> distinct-elems!84!val!5
+  T@U!val!50 -> distinct-elems!84!val!50
+  T@U!val!51 -> distinct-elems!84!val!51
+  T@U!val!52 -> distinct-elems!84!val!52
+  T@U!val!53 -> distinct-elems!84!val!53
+  T@U!val!54 -> distinct-elems!84!val!54
+  T@U!val!55 -> distinct-elems!84!val!55
+  T@U!val!56 -> distinct-elems!84!val!56
+  T@U!val!6 -> distinct-elems!84!val!6
+  T@U!val!7 -> distinct-elems!84!val!7
+  T@U!val!8 -> distinct-elems!84!val!8
+  T@U!val!9 -> distinct-elems!84!val!9
+  else -> distinct-elems!84!val!0
+}
+Div -> {
+  else -> 0
+}
+DtRank -> {
+  else -> 0
+}
+dtype -> {
+  else -> T@U!val!0
+}
+FDim -> {
+  T@U!val!22 -> 0
+  else -> 0
+}
+FieldOfDecl -> {
+  else -> T@U!val!0
+}
+FieldType -> {
+  T@T!val!2 -> T@T!val!9
+  else -> T@T!val!9
+}
+FieldTypeInv0 -> {
+  T@T!val!9 -> T@T!val!2
+  else -> T@T!val!2
+}
+Handle0 -> {
+  else -> T@U!val!0
+}
+Handle1 -> {
+  else -> T@U!val!0
+}
+IMap#Build -> {
+  else -> T@U!val!0
+}
+IMap#Domain -> {
+  else -> T@U!val!0
+}
+IMap#Elements -> {
+  else -> T@U!val!0
+}
+IMap#Empty -> {
+  else -> T@U!val!0
+}
+IMap#Equal -> {
+  else -> false
+}
+IMap#Glue -> {
+  else -> T@U!val!0
+}
+IMap#Items -> {
+  else -> T@U!val!0
+}
+IMap#Merge -> {
+  else -> T@U!val!0
+}
+IMap#Subtract -> {
+  else -> T@U!val!0
+}
+IMap#Values -> {
+  else -> T@U!val!0
+}
+IMapType -> {
+  else -> T@T!val!0
+}
+IMapTypeInv0 -> {
+  else -> T@T!val!0
+}
+IMapTypeInv1 -> {
+  else -> T@T!val!0
+}
+IndexField -> {
+  else -> T@U!val!0
+}
+IndexField_Inverse -> {
+  else -> 0
+}
+int_2_U -> {
+  else -> T@U!val!0
+}
+INTERNAL_add_boogie -> {
+  else -> 0
+}
+INTERNAL_div_boogie -> {
+  else -> 0
+}
+INTERNAL_ge_boogie -> {
+  else -> false
+}
+INTERNAL_gt_boogie -> {
+  else -> false
+}
+INTERNAL_le_boogie -> {
+  else -> false
+}
+INTERNAL_lt_boogie -> {
+  else -> false
+}
+INTERNAL_mod_boogie -> {
+  else -> 0
+}
+INTERNAL_mul_boogie -> {
+  else -> 0
+}
+INTERNAL_sub_boogie -> {
+  else -> 0
+}
+Inv0_TBitvector -> {
+  else -> 0
+}
+Inv0_TIMap -> {
+  else -> T@U!val!0
+}
+Inv0_TISet -> {
+  else -> T@U!val!0
+}
+Inv0_TMap -> {
+  else -> T@U!val!0
+}
+Inv0_TMultiSet -> {
+  else -> T@U!val!0
+}
+Inv0_TSeq -> {
+  else -> T@U!val!0
+}
+Inv0_TSet -> {
+  else -> T@U!val!0
+}
+Inv1_TIMap -> {
+  else -> T@U!val!0
+}
+Inv1_TMap -> {
+  else -> T@U!val!0
+}
+ISet#Difference -> {
+  else -> T@U!val!0
+}
+ISet#Disjoint -> {
+  else -> false
+}
+ISet#Empty -> {
+  else -> T@U!val!0
+}
+ISet#Equal -> {
+  else -> false
+}
+ISet#Intersection -> {
+  else -> T@U!val!0
+}
+ISet#Subset -> {
+  else -> false
+}
+ISet#Union -> {
+  else -> T@U!val!0
+}
+ISet#UnionOne -> {
+  else -> T@U!val!0
+}
+lambda#0 -> {
+  T@U!val!60 T@U!val!65 T@U!val!22 false -> T@U!val!66
+  else -> T@U!val!66
+}
+Lit -> {
+  false -> false
+  T@U!val!63 -> T@U!val!63
+  else -> T@U!val!63
+}
+LitInt -> {
+  else -> 0
+}
+LitReal -> {
+  else -> 0.0
+}
+Map#Build -> {
+  else -> T@U!val!0
+}
+Map#Card -> {
+  else -> 0
+}
+Map#Disjoint -> {
+  else -> false
+}
+Map#Domain -> {
+  else -> T@U!val!0
+}
+Map#Elements -> {
+  else -> T@U!val!0
+}
+Map#Empty -> {
+  else -> T@U!val!0
+}
+Map#Equal -> {
+  else -> false
+}
+Map#Glue -> {
+  else -> T@U!val!0
+}
+Map#Items -> {
+  else -> T@U!val!0
+}
+Map#Merge -> {
+  else -> T@U!val!0
+}
+Map#Subtract -> {
+  else -> T@U!val!0
+}
+Map#Values -> {
+  else -> T@U!val!0
+}
+MapType -> {
+  else -> T@T!val!0
+}
+MapType0Select -> {
+  else -> T@U!val!0
+}
+MapType0Store -> {
+  else -> T@U!val!0
+}
+MapType0Type -> {
+  T@T!val!16 T@T!val!15 -> T@T!val!19
+  else -> T@T!val!19
+}
+MapType0TypeInv0 -> {
+  T@T!val!19 -> T@T!val!16
+  else -> T@T!val!16
+}
+MapType0TypeInv1 -> {
+  T@T!val!19 -> T@T!val!15
+  else -> T@T!val!15
+}
+MapType1Select -> {
+  else -> T@U!val!0
+}
+MapType1Store -> {
+  else -> T@U!val!0
+}
+MapType2Select -> {
+  else -> T@U!val!0
+}
+MapType2Store -> {
+  else -> T@U!val!0
+}
+MapType2Type -> {
+  else -> T@T!val!0
+}
+MapType2TypeInv0 -> {
+  else -> T@T!val!0
+}
+MapType2TypeInv1 -> {
+  else -> T@T!val!0
+}
+MapType2TypeInv2 -> {
+  else -> T@T!val!0
+}
+MapType3Select -> {
+  else -> T@U!val!0
+}
+MapType3Store -> {
+  else -> T@U!val!0
+}
+MapType3Type -> {
+  T@T!val!16 T@T!val!2 -> T@T!val!21
+  else -> T@T!val!21
+}
+MapType3TypeInv0 -> {
+  T@T!val!21 -> T@T!val!16
+  else -> T@T!val!16
+}
+MapType3TypeInv1 -> {
+  T@T!val!21 -> T@T!val!2
+  else -> T@T!val!2
+}
+MapTypeInv0 -> {
+  else -> T@T!val!0
+}
+MapTypeInv1 -> {
+  else -> T@T!val!0
+}
+Math#clip -> {
+  else -> 0
+}
+Math#min -> {
+  else -> 0
+}
+Mod -> {
+  else -> 0
+}
+Mul -> {
+  else -> 0
+}
+MultiIndexField -> {
+  else -> T@U!val!0
+}
+MultiIndexField_Inverse0 -> {
+  else -> T@U!val!0
+}
+MultiIndexField_Inverse1 -> {
+  else -> 0
+}
+MultiSet#Card -> {
+  else -> 0
+}
+MultiSet#Difference -> {
+  else -> T@U!val!0
+}
+MultiSet#Disjoint -> {
+  else -> false
+}
+MultiSet#Empty -> {
+  else -> T@U!val!0
+}
+MultiSet#Equal -> {
+  else -> false
+}
+MultiSet#FromSeq -> {
+  else -> T@U!val!0
+}
+MultiSet#FromSet -> {
+  else -> T@U!val!0
+}
+MultiSet#Intersection -> {
+  else -> T@U!val!0
+}
+MultiSet#Singleton -> {
+  else -> T@U!val!0
+}
+MultiSet#Subset -> {
+  else -> false
+}
+MultiSet#Union -> {
+  else -> T@U!val!0
+}
+MultiSet#UnionOne -> {
+  else -> T@U!val!0
+}
+ORD#FromNat -> {
+  else -> T@U!val!0
+}
+ORD#IsNat -> {
+  else -> false
+}
+ORD#Less -> {
+  else -> false
+}
+ORD#LessThanLimit -> {
+  else -> false
+}
+ORD#Minus -> {
+  else -> T@U!val!0
+}
+ORD#Offset -> {
+  else -> 0
+}
+ORD#Plus -> {
+  else -> T@U!val!0
+}
+q@Int -> {
+  else -> 0
+}
+q@Real -> {
+  else -> 0.0
+}
+Reads0 -> {
+  else -> T@U!val!0
+}
+Reads1 -> {
+  else -> T@U!val!0
+}
+real_2_U -> {
+  else -> T@U!val!0
+}
+real_pow -> {
+  else -> 0.0
+}
+regex_2_U -> {
+  else -> T@U!val!0
+}
+Requires0 -> {
+  else -> false
+}
+Requires1 -> {
+  else -> false
+}
+rmode_2_U -> {
+  else -> T@U!val!0
+}
+Seq#Append -> {
+  else -> T@U!val!0
+}
+Seq#Build -> {
+  else -> T@U!val!0
+}
+Seq#Build_inv0 -> {
+  else -> T@U!val!0
+}
+Seq#Build_inv1 -> {
+  else -> T@U!val!0
+}
+Seq#Contains -> {
+  else -> false
+}
+Seq#Create -> {
+  else -> T@U!val!0
+}
+Seq#Drop -> {
+  else -> T@U!val!0
+}
+Seq#Empty -> {
+  else -> T@U!val!0
+}
+Seq#Equal -> {
+  else -> false
+}
+Seq#FromArray -> {
+  else -> T@U!val!0
+}
+Seq#Index -> {
+  else -> T@U!val!0
+}
+Seq#Length -> {
+  else -> 0
+}
+Seq#Rank -> {
+  else -> 0
+}
+Seq#SameUntil -> {
+  else -> false
+}
+Seq#Singleton -> {
+  else -> T@U!val!0
+}
+Seq#Take -> {
+  else -> T@U!val!0
+}
+Seq#Update -> {
+  else -> T@U!val!0
+}
+SeqType -> {
+  else -> T@T!val!0
+}
+SeqTypeInv0 -> {
+  else -> T@T!val!0
+}
+Set#Card -> {
+  else -> 0
+}
+Set#Difference -> {
+  else -> T@U!val!0
+}
+Set#Disjoint -> {
+  else -> false
+}
+Set#Empty -> {
+  else -> T@U!val!0
+}
+Set#Equal -> {
+  else -> false
+}
+Set#Intersection -> {
+  else -> T@U!val!0
+}
+Set#Singleton -> {
+  else -> T@U!val!0
+}
+Set#Subset -> {
+  else -> false
+}
+Set#Union -> {
+  else -> T@U!val!0
+}
+Set#UnionOne -> {
+  else -> T@U!val!0
+}
+SetRef_to_SetBox -> {
+  else -> T@U!val!0
+}
+string_2_U -> {
+  else -> T@U!val!0
+}
+Sub -> {
+  else -> 0
+}
+Tag -> {
+  T@U!val!0 -> T@U!val!5
+  T@U!val!1 -> T@U!val!6
+  T@U!val!2 -> T@U!val!7
+  T@U!val!3 -> T@U!val!8
+  T@U!val!4 -> T@U!val!9
+  T@U!val!57 -> T@U!val!26
+  T@U!val!59 -> T@U!val!24
+  T@U!val!61 -> T@U!val!27
+  T@U!val!62 -> T@U!val!41
+  T@U!val!64 -> T@U!val!44
+  else -> T@U!val!5
+}
+TagFamily -> {
+  T@U!val!57 -> T@U!val!46
+  T@U!val!59 -> T@U!val!45
+  T@U!val!61 -> T@U!val!46
+  T@U!val!62 -> T@U!val!55
+  T@U!val!64 -> T@U!val!56
+  else -> T@U!val!46
+}
+TBitvector -> {
+  else -> T@U!val!0
+}
+Tclass._System.___hFunc0 -> {
+  else -> T@U!val!0
+}
+Tclass._System.___hFunc0_0 -> {
+  else -> T@U!val!0
+}
+Tclass._System.___hFunc1 -> {
+  else -> T@U!val!0
+}
+Tclass._System.___hFunc1_0 -> {
+  else -> T@U!val!0
+}
+Tclass._System.___hFunc1_1 -> {
+  else -> T@U!val!0
+}
+Tclass._System.___hPartialFunc0 -> {
+  else -> T@U!val!0
+}
+Tclass._System.___hPartialFunc0_0 -> {
+  else -> T@U!val!0
+}
+Tclass._System.___hPartialFunc1 -> {
+  else -> T@U!val!0
+}
+Tclass._System.___hPartialFunc1_0 -> {
+  else -> T@U!val!0
+}
+Tclass._System.___hPartialFunc1_1 -> {
+  else -> T@U!val!0
+}
+Tclass._System.___hTotalFunc0 -> {
+  else -> T@U!val!0
+}
+Tclass._System.___hTotalFunc0_0 -> {
+  else -> T@U!val!0
+}
+Tclass._System.___hTotalFunc1 -> {
+  else -> T@U!val!0
+}
+Tclass._System.___hTotalFunc1_0 -> {
+  else -> T@U!val!0
+}
+Tclass._System.___hTotalFunc1_1 -> {
+  else -> T@U!val!0
+}
+Tclass._System.array -> {
+  else -> T@U!val!0
+}
+Tclass._System.array_0 -> {
+  else -> T@U!val!0
+}
+Tclass._System.array? -> {
+  else -> T@U!val!0
+}
+Tclass._System.array?_0 -> {
+  else -> T@U!val!0
+}
+Tclass._System.Tuple2 -> {
+  else -> T@U!val!0
+}
+Tclass._System.Tuple2_0 -> {
+  else -> T@U!val!0
+}
+Tclass._System.Tuple2_1 -> {
+  else -> T@U!val!0
+}
+tickleBool -> {
+  false -> true
+  true -> true
+  else -> true
+}
+TIMap -> {
+  else -> T@U!val!0
+}
+TISet -> {
+  else -> T@U!val!0
+}
+TMap -> {
+  else -> T@U!val!0
+}
+TMultiSet -> {
+  else -> T@U!val!0
+}
+TSeq -> {
+  else -> T@U!val!0
+}
+TSet -> {
+  else -> T@U!val!0
+}
+type -> {
+  false -> T@T!val!2
+  T@U!val!0 -> T@T!val!6
+  T@U!val!1 -> T@T!val!6
+  T@U!val!10 -> T@T!val!7
+  T@U!val!11 -> T@T!val!7
+  T@U!val!12 -> T@T!val!7
+  T@U!val!13 -> T@T!val!7
+  T@U!val!14 -> T@T!val!7
+  T@U!val!15 -> T@T!val!7
+  T@U!val!16 -> T@T!val!7
+  T@U!val!17 -> T@T!val!8
+  T@U!val!18 -> T@T!val!8
+  T@U!val!19 -> T@T!val!8
+  T@U!val!2 -> T@T!val!6
+  T@U!val!20 -> T@T!val!8
+  T@U!val!21 -> T@T!val!8
+  T@U!val!22 -> T@T!val!9
+  T@U!val!23 -> T@T!val!10
+  T@U!val!24 -> T@T!val!7
+  T@U!val!25 -> T@T!val!8
+  T@U!val!26 -> T@T!val!7
+  T@U!val!27 -> T@T!val!7
+  T@U!val!28 -> T@T!val!8
+  T@U!val!29 -> T@T!val!7
+  T@U!val!3 -> T@T!val!6
+  T@U!val!30 -> T@T!val!7
+  T@U!val!31 -> T@T!val!7
+  T@U!val!32 -> T@T!val!7
+  T@U!val!33 -> T@T!val!7
+  T@U!val!34 -> T@T!val!7
+  T@U!val!35 -> T@T!val!7
+  T@U!val!36 -> T@T!val!7
+  T@U!val!37 -> T@T!val!11
+  T@U!val!38 -> T@T!val!7
+  T@U!val!39 -> T@T!val!8
+  T@U!val!4 -> T@T!val!6
+  T@U!val!40 -> T@T!val!11
+  T@U!val!41 -> T@T!val!7
+  T@U!val!42 -> T@T!val!8
+  T@U!val!43 -> T@T!val!8
+  T@U!val!44 -> T@T!val!7
+  T@U!val!45 -> T@T!val!12
+  T@U!val!46 -> T@T!val!12
+  T@U!val!47 -> T@T!val!12
+  T@U!val!48 -> T@T!val!12
+  T@U!val!49 -> T@T!val!12
+  T@U!val!5 -> T@T!val!7
+  T@U!val!50 -> T@T!val!12
+  T@U!val!51 -> T@T!val!12
+  T@U!val!52 -> T@T!val!12
+  T@U!val!53 -> T@T!val!12
+  T@U!val!54 -> T@T!val!12
+  T@U!val!55 -> T@T!val!12
+  T@U!val!56 -> T@T!val!12
+  T@U!val!57 -> T@T!val!6
+  T@U!val!58 -> T@T!val!19
+  T@U!val!59 -> T@T!val!6
+  T@U!val!6 -> T@T!val!7
+  T@U!val!60 -> T@T!val!16
+  T@U!val!61 -> T@T!val!6
+  T@U!val!62 -> T@T!val!6
+  T@U!val!63 -> T@T!val!17
+  T@U!val!64 -> T@T!val!6
+  T@U!val!65 -> T@T!val!19
+  T@U!val!66 -> T@T!val!21
+  T@U!val!7 -> T@T!val!7
+  T@U!val!8 -> T@T!val!7
+  T@U!val!9 -> T@T!val!7
+  else -> T@T!val!7
+}
+TypeTuple -> {
+  else -> T@U!val!0
+}
+TypeTupleCar -> {
+  else -> T@U!val!0
+}
+TypeTupleCdr -> {
+  else -> T@U!val!0
+}
+U_2_bool -> {
+  false -> false
+  else -> false
+}
+U_2_int -> {
+  else -> 0
+}
+U_2_real -> {
+  else -> 0.0
+}
+U_2_regex -> {
+  else -> (str.to.re (""))
+}
+U_2_rmode -> {
+  else -> (roundTowardZero)
+}
+U_2_string -> {
+  else -> ("")
+}
+UOrdering2 -> {
+  else -> false
+}
+UOrdering3 -> {
+  else -> false
+}
+*** STATE <initial>
+  $_Frame -> 
+  $_reverifyPost -> 
+  $Heap -> T@U!val!65
+  $Tick -> 
+  a#0 -> 11
+  b#0 -> 6
+  c#0 -> 
+  defass#c#0 -> 
+*** END_STATE
+*** STATE /workspaces/dafny/string_project/str_recurse.dfy(5,2): initial state
+  $_Frame -> T@U!val!66
+*** END_STATE
+*** END_MODEL
+<no file>(1500,4): Error: This assertion might not hold.
+Execution trace:
+    (1609,3): anon0
+Augmented execution trace:
+Impl | Impl$$M.__default.foo | 11 | 5
+Types | int | int
+
+
+*** MODEL
+#_System._tuple#0._#Make0 -> T@U!val!63
+##_System._tuple#0._#Make0 -> T@U!val!40
+##_System._tuple#2._#Make2 -> T@U!val!37
+$_Frame -> 
+$_Frame@0 -> T@U!val!66
+$_reverifyPost -> 
+$$Language$Dafny -> true
+$FunctionContextHeight -> 0
+$Heap -> T@U!val!65
+$OneHeap -> T@U!val!58
+$Tick -> 
+a#0 -> 11
+alloc -> T@U!val!22
+allocName -> T@U!val!23
+b#0 -> 5
+boolType -> T@T!val!2
+BoxType -> T@T!val!13
+c#0 -> 
+charType -> T@T!val!14
+class._System.array? -> T@U!val!28
+class._System.bool -> T@U!val!18
+class._System.int -> T@U!val!17
+class._System.multiset -> T@U!val!21
+class._System.object? -> T@U!val!25
+class._System.seq -> T@U!val!20
+class._System.set -> T@U!val!19
+class._System.Tuple0 -> T@U!val!42
+class._System.Tuple2 -> T@U!val!39
+class.M.__default -> T@U!val!43
+ClassNameType -> T@T!val!8
+DatatypeTypeType -> T@T!val!17
+defass#c#0 -> 
+DtCtorIdType -> T@T!val!11
+HandleTypeType -> T@T!val!20
+intType -> T@T!val!0
+LayerTypeType -> T@T!val!18
+MapType1Type -> T@T!val!15
+NameFamilyType -> T@T!val!10
+null -> T@U!val!60
+proxy!143 -> true
+realType -> T@T!val!1
+refType -> T@T!val!16
+regexType -> T@T!val!5
+rmodeType -> T@T!val!3
+stringType -> T@T!val!4
+TagBool -> T@U!val!5
+TagChar -> T@U!val!6
+TagClass -> T@U!val!16
+Tagclass._System.___hFunc0 -> T@U!val!34
+Tagclass._System.___hFunc1 -> T@U!val!31
+Tagclass._System.___hPartialFunc0 -> T@U!val!35
+Tagclass._System.___hPartialFunc1 -> T@U!val!32
+Tagclass._System.___hTotalFunc0 -> T@U!val!36
+Tagclass._System.___hTotalFunc1 -> T@U!val!33
+Tagclass._System.array -> T@U!val!30
+Tagclass._System.array? -> T@U!val!29
+Tagclass._System.nat -> T@U!val!24
+Tagclass._System.object -> T@U!val!27
+Tagclass._System.object? -> T@U!val!26
+Tagclass._System.Tuple0 -> T@U!val!41
+Tagclass._System.Tuple2 -> T@U!val!38
+Tagclass.M.__default -> T@U!val!44
+TagIMap -> T@U!val!15
+TagInt -> T@U!val!7
+TagISet -> T@U!val!11
+TagMap -> T@U!val!14
+TagMultiSet -> T@U!val!12
+TagORDINAL -> T@U!val!9
+TagReal -> T@U!val!8
+TagSeq -> T@U!val!13
+TagSet -> T@U!val!10
+TBool -> T@U!val!0
+TChar -> T@U!val!1
+Tclass._System.nat -> T@U!val!59
+Tclass._System.object -> T@U!val!61
+Tclass._System.object? -> T@U!val!57
+Tclass._System.Tuple0 -> T@U!val!62
+Tclass.M.__default -> T@U!val!64
+TInt -> T@U!val!2
+TORDINAL -> T@U!val!4
+TReal -> T@U!val!3
+tytagFamily$_#Func0 -> T@U!val!51
+tytagFamily$_#Func1 -> T@U!val!48
+tytagFamily$_#PartialFunc0 -> T@U!val!52
+tytagFamily$_#PartialFunc1 -> T@U!val!49
+tytagFamily$_#TotalFunc0 -> T@U!val!53
+tytagFamily$_#TotalFunc1 -> T@U!val!50
+tytagFamily$_default -> T@U!val!56
+tytagFamily$_tuple#0 -> T@U!val!55
+tytagFamily$_tuple#2 -> T@U!val!54
+tytagFamily$array -> T@U!val!47
+tytagFamily$nat -> T@U!val!45
+tytagFamily$object -> T@U!val!46
+TyTagFamilyType -> T@T!val!12
+TyTagType -> T@T!val!7
+TyType -> T@T!val!6
+unique-value!100 -> distinct-elems!84!val!14
+unique-value!101 -> distinct-elems!84!val!15
+unique-value!102 -> distinct-elems!84!val!16
+unique-value!103 -> distinct-elems!84!val!17
+unique-value!104 -> distinct-elems!84!val!18
+unique-value!105 -> distinct-elems!84!val!19
+unique-value!106 -> distinct-elems!84!val!20
+unique-value!107 -> distinct-elems!84!val!21
+unique-value!108 -> distinct-elems!84!val!22
+unique-value!109 -> distinct-elems!84!val!23
+unique-value!110 -> distinct-elems!84!val!24
+unique-value!111 -> distinct-elems!84!val!25
+unique-value!112 -> distinct-elems!84!val!26
+unique-value!113 -> distinct-elems!84!val!27
+unique-value!114 -> distinct-elems!84!val!28
+unique-value!115 -> distinct-elems!84!val!29
+unique-value!116 -> distinct-elems!84!val!30
+unique-value!117 -> distinct-elems!84!val!31
+unique-value!118 -> distinct-elems!84!val!32
+unique-value!119 -> distinct-elems!84!val!33
+unique-value!120 -> distinct-elems!84!val!34
+unique-value!121 -> distinct-elems!84!val!35
+unique-value!122 -> distinct-elems!84!val!36
+unique-value!123 -> distinct-elems!84!val!37
+unique-value!124 -> distinct-elems!84!val!38
+unique-value!125 -> distinct-elems!84!val!39
+unique-value!126 -> distinct-elems!84!val!40
+unique-value!127 -> distinct-elems!84!val!41
+unique-value!128 -> distinct-elems!84!val!42
+unique-value!129 -> distinct-elems!84!val!43
+unique-value!130 -> distinct-elems!84!val!44
+unique-value!131 -> distinct-elems!84!val!45
+unique-value!132 -> distinct-elems!84!val!46
+unique-value!133 -> distinct-elems!84!val!47
+unique-value!134 -> distinct-elems!84!val!48
+unique-value!135 -> distinct-elems!84!val!49
+unique-value!136 -> distinct-elems!84!val!50
+unique-value!137 -> distinct-elems!84!val!51
+unique-value!138 -> distinct-elems!84!val!52
+unique-value!139 -> distinct-elems!84!val!53
+unique-value!140 -> distinct-elems!84!val!54
+unique-value!141 -> distinct-elems!84!val!55
+unique-value!142 -> distinct-elems!84!val!56
+unique-value!86 -> distinct-elems!84!val!0
+unique-value!87 -> distinct-elems!84!val!1
+unique-value!88 -> distinct-elems!84!val!2
+unique-value!89 -> distinct-elems!84!val!3
+unique-value!90 -> distinct-elems!84!val!4
+unique-value!91 -> distinct-elems!84!val!5
+unique-value!92 -> distinct-elems!84!val!6
+unique-value!93 -> distinct-elems!84!val!7
+unique-value!94 -> distinct-elems!84!val!8
+unique-value!95 -> distinct-elems!84!val!9
+unique-value!96 -> distinct-elems!84!val!10
+unique-value!97 -> distinct-elems!84!val!11
+unique-value!98 -> distinct-elems!84!val!12
+unique-value!99 -> distinct-elems!84!val!13
+_System.array.Length -> {
+  else -> 0
+}
+_System.Tuple0.___hMake0_q -> {
+  else -> false
+}
+_System.Tuple0#Equal -> {
+  else -> false
+}
+_System.Tuple2.___hMake2_q -> {
+  else -> false
+}
+_System.Tuple2._0 -> {
+  else -> T@U!val!0
+}
+_System.Tuple2._1 -> {
+  else -> T@U!val!0
+}
+_System.Tuple2#Equal -> {
+  else -> false
+}
+#_System._tuple#2._#Make2 -> {
+  else -> T@U!val!0
+}
+$Box -> {
+  else -> T@U!val!0
+}
+$HeapSucc -> {
+  else -> false
+}
+$HeapSuccGhost -> {
+  else -> false
+}
+$Is -> {
+  T@U!val!63 T@U!val!62 -> true
+  else -> true
+}
+$IsA#_System.Tuple0 -> {
+  else -> false
+}
+$IsA#_System.Tuple2 -> {
+  else -> false
+}
+$IsAlloc -> {
+  else -> false
+}
+$IsAllocBox -> {
+  else -> false
+}
+$IsBox -> {
+  else -> false
+}
+$IsGhostField -> {
+  T@U!val!22 -> false
+  else -> false
+}
+$IsGoodHeap -> {
+  T@U!val!58 -> true
+  T@U!val!65 -> true
+  else -> true
+}
+$IsGoodMultiSet -> {
+  else -> false
+}
+$IsHeapAnchor -> {
+  T@U!val!65 -> true
+  else -> true
+}
+$LS -> {
+  else -> T@U!val!0
+}
+$Unbox -> {
+  else -> T@U!val!0
+}
+Add -> {
+  else -> 0
+}
+Apply0 -> {
+  else -> T@U!val!0
+}
+Apply1 -> {
+  else -> T@U!val!0
+}
+AtLayer -> {
+  else -> T@U!val!0
+}
+bool_2_U -> {
+  false -> false
+  else -> false
+}
+BoxRank -> {
+  else -> 0
+}
+char#FromInt -> {
+  else -> T@U!val!0
+}
+char#Minus -> {
+  else -> T@U!val!0
+}
+char#Plus -> {
+  else -> T@U!val!0
+}
+char#ToInt -> {
+  else -> 0
+}
+ControlFlow -> {
+  0 0 -> 63373
+  0 54326 -> (- 63460)
+  0 63373 -> 54326
+  else -> 63373
+}
+Ctor -> {
+  T@T!val!0 -> 0
+  T@T!val!1 -> 1
+  T@T!val!10 -> 10
+  T@T!val!11 -> 11
+  T@T!val!12 -> 12
+  T@T!val!13 -> 13
+  T@T!val!14 -> 14
+  T@T!val!15 -> 19
+  T@T!val!16 -> 20
+  T@T!val!17 -> 21
+  T@T!val!18 -> 22
+  T@T!val!19 -> 15
+  T@T!val!2 -> 2
+  T@T!val!20 -> 23
+  T@T!val!21 -> 25
+  T@T!val!3 -> 3
+  T@T!val!4 -> 4
+  T@T!val!5 -> 5
+  T@T!val!6 -> 6
+  T@T!val!7 -> 7
+  T@T!val!8 -> 8
+  T@T!val!9 -> 9
+  else -> 0
+}
+DatatypeCtorId -> {
+  T@U!val!63 -> T@U!val!40
+  else -> T@U!val!40
+}
+DeclName -> {
+  T@U!val!22 -> T@U!val!23
+  else -> T@U!val!23
+}
+DeclType -> {
+  else -> T@U!val!0
+}
+distinct-aux-f!!85 -> {
+  T@U!val!0 -> distinct-elems!84!val!0
+  T@U!val!1 -> distinct-elems!84!val!1
+  T@U!val!10 -> distinct-elems!84!val!10
+  T@U!val!11 -> distinct-elems!84!val!11
+  T@U!val!12 -> distinct-elems!84!val!12
+  T@U!val!13 -> distinct-elems!84!val!13
+  T@U!val!14 -> distinct-elems!84!val!14
+  T@U!val!15 -> distinct-elems!84!val!15
+  T@U!val!16 -> distinct-elems!84!val!16
+  T@U!val!17 -> distinct-elems!84!val!17
+  T@U!val!18 -> distinct-elems!84!val!18
+  T@U!val!19 -> distinct-elems!84!val!19
+  T@U!val!2 -> distinct-elems!84!val!2
+  T@U!val!20 -> distinct-elems!84!val!20
+  T@U!val!21 -> distinct-elems!84!val!21
+  T@U!val!22 -> distinct-elems!84!val!22
+  T@U!val!23 -> distinct-elems!84!val!23
+  T@U!val!24 -> distinct-elems!84!val!24
+  T@U!val!25 -> distinct-elems!84!val!25
+  T@U!val!26 -> distinct-elems!84!val!26
+  T@U!val!27 -> distinct-elems!84!val!27
+  T@U!val!28 -> distinct-elems!84!val!28
+  T@U!val!29 -> distinct-elems!84!val!29
+  T@U!val!3 -> distinct-elems!84!val!3
+  T@U!val!30 -> distinct-elems!84!val!30
+  T@U!val!31 -> distinct-elems!84!val!31
+  T@U!val!32 -> distinct-elems!84!val!32
+  T@U!val!33 -> distinct-elems!84!val!33
+  T@U!val!34 -> distinct-elems!84!val!34
+  T@U!val!35 -> distinct-elems!84!val!35
+  T@U!val!36 -> distinct-elems!84!val!36
+  T@U!val!37 -> distinct-elems!84!val!37
+  T@U!val!38 -> distinct-elems!84!val!38
+  T@U!val!39 -> distinct-elems!84!val!39
+  T@U!val!4 -> distinct-elems!84!val!4
+  T@U!val!40 -> distinct-elems!84!val!40
+  T@U!val!41 -> distinct-elems!84!val!41
+  T@U!val!42 -> distinct-elems!84!val!42
+  T@U!val!43 -> distinct-elems!84!val!43
+  T@U!val!44 -> distinct-elems!84!val!44
+  T@U!val!45 -> distinct-elems!84!val!45
+  T@U!val!46 -> distinct-elems!84!val!46
+  T@U!val!47 -> distinct-elems!84!val!47
+  T@U!val!48 -> distinct-elems!84!val!48
+  T@U!val!49 -> distinct-elems!84!val!49
+  T@U!val!5 -> distinct-elems!84!val!5
+  T@U!val!50 -> distinct-elems!84!val!50
+  T@U!val!51 -> distinct-elems!84!val!51
+  T@U!val!52 -> distinct-elems!84!val!52
+  T@U!val!53 -> distinct-elems!84!val!53
+  T@U!val!54 -> distinct-elems!84!val!54
+  T@U!val!55 -> distinct-elems!84!val!55
+  T@U!val!56 -> distinct-elems!84!val!56
+  T@U!val!6 -> distinct-elems!84!val!6
+  T@U!val!7 -> distinct-elems!84!val!7
+  T@U!val!8 -> distinct-elems!84!val!8
+  T@U!val!9 -> distinct-elems!84!val!9
+  else -> distinct-elems!84!val!0
+}
+Div -> {
+  else -> 0
+}
+DtRank -> {
+  else -> 0
+}
+dtype -> {
+  else -> T@U!val!0
+}
+FDim -> {
+  T@U!val!22 -> 0
+  else -> 0
+}
+FieldOfDecl -> {
+  else -> T@U!val!0
+}
+FieldType -> {
+  T@T!val!2 -> T@T!val!9
+  else -> T@T!val!9
+}
+FieldTypeInv0 -> {
+  T@T!val!9 -> T@T!val!2
+  else -> T@T!val!2
+}
+Handle0 -> {
+  else -> T@U!val!0
+}
+Handle1 -> {
+  else -> T@U!val!0
+}
+IMap#Build -> {
+  else -> T@U!val!0
+}
+IMap#Domain -> {
+  else -> T@U!val!0
+}
+IMap#Elements -> {
+  else -> T@U!val!0
+}
+IMap#Empty -> {
+  else -> T@U!val!0
+}
+IMap#Equal -> {
+  else -> false
+}
+IMap#Glue -> {
+  else -> T@U!val!0
+}
+IMap#Items -> {
+  else -> T@U!val!0
+}
+IMap#Merge -> {
+  else -> T@U!val!0
+}
+IMap#Subtract -> {
+  else -> T@U!val!0
+}
+IMap#Values -> {
+  else -> T@U!val!0
+}
+IMapType -> {
+  else -> T@T!val!0
+}
+IMapTypeInv0 -> {
+  else -> T@T!val!0
+}
+IMapTypeInv1 -> {
+  else -> T@T!val!0
+}
+IndexField -> {
+  else -> T@U!val!0
+}
+IndexField_Inverse -> {
+  else -> 0
+}
+int_2_U -> {
+  else -> T@U!val!0
+}
+INTERNAL_add_boogie -> {
+  else -> 0
+}
+INTERNAL_div_boogie -> {
+  else -> 0
+}
+INTERNAL_ge_boogie -> {
+  else -> false
+}
+INTERNAL_gt_boogie -> {
+  else -> false
+}
+INTERNAL_le_boogie -> {
+  else -> false
+}
+INTERNAL_lt_boogie -> {
+  else -> false
+}
+INTERNAL_mod_boogie -> {
+  else -> 0
+}
+INTERNAL_mul_boogie -> {
+  else -> 0
+}
+INTERNAL_sub_boogie -> {
+  else -> 0
+}
+Inv0_TBitvector -> {
+  else -> 0
+}
+Inv0_TIMap -> {
+  else -> T@U!val!0
+}
+Inv0_TISet -> {
+  else -> T@U!val!0
+}
+Inv0_TMap -> {
+  else -> T@U!val!0
+}
+Inv0_TMultiSet -> {
+  else -> T@U!val!0
+}
+Inv0_TSeq -> {
+  else -> T@U!val!0
+}
+Inv0_TSet -> {
+  else -> T@U!val!0
+}
+Inv1_TIMap -> {
+  else -> T@U!val!0
+}
+Inv1_TMap -> {
+  else -> T@U!val!0
+}
+ISet#Difference -> {
+  else -> T@U!val!0
+}
+ISet#Disjoint -> {
+  else -> false
+}
+ISet#Empty -> {
+  else -> T@U!val!0
+}
+ISet#Equal -> {
+  else -> false
+}
+ISet#Intersection -> {
+  else -> T@U!val!0
+}
+ISet#Subset -> {
+  else -> false
+}
+ISet#Union -> {
+  else -> T@U!val!0
+}
+ISet#UnionOne -> {
+  else -> T@U!val!0
+}
+lambda#0 -> {
+  T@U!val!60 T@U!val!65 T@U!val!22 false -> T@U!val!66
+  else -> T@U!val!66
+}
+Lit -> {
+  false -> false
+  T@U!val!63 -> T@U!val!63
+  else -> T@U!val!63
+}
+LitInt -> {
+  else -> 0
+}
+LitReal -> {
+  else -> 0.0
+}
+Map#Build -> {
+  else -> T@U!val!0
+}
+Map#Card -> {
+  else -> 0
+}
+Map#Disjoint -> {
+  else -> false
+}
+Map#Domain -> {
+  else -> T@U!val!0
+}
+Map#Elements -> {
+  else -> T@U!val!0
+}
+Map#Empty -> {
+  else -> T@U!val!0
+}
+Map#Equal -> {
+  else -> false
+}
+Map#Glue -> {
+  else -> T@U!val!0
+}
+Map#Items -> {
+  else -> T@U!val!0
+}
+Map#Merge -> {
+  else -> T@U!val!0
+}
+Map#Subtract -> {
+  else -> T@U!val!0
+}
+Map#Values -> {
+  else -> T@U!val!0
+}
+MapType -> {
+  else -> T@T!val!0
+}
+MapType0Select -> {
+  else -> T@U!val!0
+}
+MapType0Store -> {
+  else -> T@U!val!0
+}
+MapType0Type -> {
+  T@T!val!16 T@T!val!15 -> T@T!val!19
+  else -> T@T!val!19
+}
+MapType0TypeInv0 -> {
+  T@T!val!19 -> T@T!val!16
+  else -> T@T!val!16
+}
+MapType0TypeInv1 -> {
+  T@T!val!19 -> T@T!val!15
+  else -> T@T!val!15
+}
+MapType1Select -> {
+  else -> T@U!val!0
+}
+MapType1Store -> {
+  else -> T@U!val!0
+}
+MapType2Select -> {
+  else -> T@U!val!0
+}
+MapType2Store -> {
+  else -> T@U!val!0
+}
+MapType2Type -> {
+  else -> T@T!val!0
+}
+MapType2TypeInv0 -> {
+  else -> T@T!val!0
+}
+MapType2TypeInv1 -> {
+  else -> T@T!val!0
+}
+MapType2TypeInv2 -> {
+  else -> T@T!val!0
+}
+MapType3Select -> {
+  else -> T@U!val!0
+}
+MapType3Store -> {
+  else -> T@U!val!0
+}
+MapType3Type -> {
+  T@T!val!16 T@T!val!2 -> T@T!val!21
+  else -> T@T!val!21
+}
+MapType3TypeInv0 -> {
+  T@T!val!21 -> T@T!val!16
+  else -> T@T!val!16
+}
+MapType3TypeInv1 -> {
+  T@T!val!21 -> T@T!val!2
+  else -> T@T!val!2
+}
+MapTypeInv0 -> {
+  else -> T@T!val!0
+}
+MapTypeInv1 -> {
+  else -> T@T!val!0
+}
+Math#clip -> {
+  else -> 0
+}
+Math#min -> {
+  else -> 0
+}
+Mod -> {
+  else -> 0
+}
+Mul -> {
+  else -> 0
+}
+MultiIndexField -> {
+  else -> T@U!val!0
+}
+MultiIndexField_Inverse0 -> {
+  else -> T@U!val!0
+}
+MultiIndexField_Inverse1 -> {
+  else -> 0
+}
+MultiSet#Card -> {
+  else -> 0
+}
+MultiSet#Difference -> {
+  else -> T@U!val!0
+}
+MultiSet#Disjoint -> {
+  else -> false
+}
+MultiSet#Empty -> {
+  else -> T@U!val!0
+}
+MultiSet#Equal -> {
+  else -> false
+}
+MultiSet#FromSeq -> {
+  else -> T@U!val!0
+}
+MultiSet#FromSet -> {
+  else -> T@U!val!0
+}
+MultiSet#Intersection -> {
+  else -> T@U!val!0
+}
+MultiSet#Singleton -> {
+  else -> T@U!val!0
+}
+MultiSet#Subset -> {
+  else -> false
+}
+MultiSet#Union -> {
+  else -> T@U!val!0
+}
+MultiSet#UnionOne -> {
+  else -> T@U!val!0
+}
+ORD#FromNat -> {
+  else -> T@U!val!0
+}
+ORD#IsNat -> {
+  else -> false
+}
+ORD#Less -> {
+  else -> false
+}
+ORD#LessThanLimit -> {
+  else -> false
+}
+ORD#Minus -> {
+  else -> T@U!val!0
+}
+ORD#Offset -> {
+  else -> 0
+}
+ORD#Plus -> {
+  else -> T@U!val!0
+}
+q@Int -> {
+  else -> 0
+}
+q@Real -> {
+  else -> 0.0
+}
+Reads0 -> {
+  else -> T@U!val!0
+}
+Reads1 -> {
+  else -> T@U!val!0
+}
+real_2_U -> {
+  else -> T@U!val!0
+}
+real_pow -> {
+  else -> 0.0
+}
+regex_2_U -> {
+  else -> T@U!val!0
+}
+Requires0 -> {
+  else -> false
+}
+Requires1 -> {
+  else -> false
+}
+rmode_2_U -> {
+  else -> T@U!val!0
+}
+Seq#Append -> {
+  else -> T@U!val!0
+}
+Seq#Build -> {
+  else -> T@U!val!0
+}
+Seq#Build_inv0 -> {
+  else -> T@U!val!0
+}
+Seq#Build_inv1 -> {
+  else -> T@U!val!0
+}
+Seq#Contains -> {
+  else -> false
+}
+Seq#Create -> {
+  else -> T@U!val!0
+}
+Seq#Drop -> {
+  else -> T@U!val!0
+}
+Seq#Empty -> {
+  else -> T@U!val!0
+}
+Seq#Equal -> {
+  else -> false
+}
+Seq#FromArray -> {
+  else -> T@U!val!0
+}
+Seq#Index -> {
+  else -> T@U!val!0
+}
+Seq#Length -> {
+  else -> 0
+}
+Seq#Rank -> {
+  else -> 0
+}
+Seq#SameUntil -> {
+  else -> false
+}
+Seq#Singleton -> {
+  else -> T@U!val!0
+}
+Seq#Take -> {
+  else -> T@U!val!0
+}
+Seq#Update -> {
+  else -> T@U!val!0
+}
+SeqType -> {
+  else -> T@T!val!0
+}
+SeqTypeInv0 -> {
+  else -> T@T!val!0
+}
+Set#Card -> {
+  else -> 0
+}
+Set#Difference -> {
+  else -> T@U!val!0
+}
+Set#Disjoint -> {
+  else -> false
+}
+Set#Empty -> {
+  else -> T@U!val!0
+}
+Set#Equal -> {
+  else -> false
+}
+Set#Intersection -> {
+  else -> T@U!val!0
+}
+Set#Singleton -> {
+  else -> T@U!val!0
+}
+Set#Subset -> {
+  else -> false
+}
+Set#Union -> {
+  else -> T@U!val!0
+}
+Set#UnionOne -> {
+  else -> T@U!val!0
+}
+SetRef_to_SetBox -> {
+  else -> T@U!val!0
+}
+string_2_U -> {
+  else -> T@U!val!0
+}
+Sub -> {
+  else -> 0
+}
+Tag -> {
+  T@U!val!0 -> T@U!val!5
+  T@U!val!1 -> T@U!val!6
+  T@U!val!2 -> T@U!val!7
+  T@U!val!3 -> T@U!val!8
+  T@U!val!4 -> T@U!val!9
+  T@U!val!57 -> T@U!val!26
+  T@U!val!59 -> T@U!val!24
+  T@U!val!61 -> T@U!val!27
+  T@U!val!62 -> T@U!val!41
+  T@U!val!64 -> T@U!val!44
+  else -> T@U!val!5
+}
+TagFamily -> {
+  T@U!val!57 -> T@U!val!46
+  T@U!val!59 -> T@U!val!45
+  T@U!val!61 -> T@U!val!46
+  T@U!val!62 -> T@U!val!55
+  T@U!val!64 -> T@U!val!56
+  else -> T@U!val!46
+}
+TBitvector -> {
+  else -> T@U!val!0
+}
+Tclass._System.___hFunc0 -> {
+  else -> T@U!val!0
+}
+Tclass._System.___hFunc0_0 -> {
+  else -> T@U!val!0
+}
+Tclass._System.___hFunc1 -> {
+  else -> T@U!val!0
+}
+Tclass._System.___hFunc1_0 -> {
+  else -> T@U!val!0
+}
+Tclass._System.___hFunc1_1 -> {
+  else -> T@U!val!0
+}
+Tclass._System.___hPartialFunc0 -> {
+  else -> T@U!val!0
+}
+Tclass._System.___hPartialFunc0_0 -> {
+  else -> T@U!val!0
+}
+Tclass._System.___hPartialFunc1 -> {
+  else -> T@U!val!0
+}
+Tclass._System.___hPartialFunc1_0 -> {
+  else -> T@U!val!0
+}
+Tclass._System.___hPartialFunc1_1 -> {
+  else -> T@U!val!0
+}
+Tclass._System.___hTotalFunc0 -> {
+  else -> T@U!val!0
+}
+Tclass._System.___hTotalFunc0_0 -> {
+  else -> T@U!val!0
+}
+Tclass._System.___hTotalFunc1 -> {
+  else -> T@U!val!0
+}
+Tclass._System.___hTotalFunc1_0 -> {
+  else -> T@U!val!0
+}
+Tclass._System.___hTotalFunc1_1 -> {
+  else -> T@U!val!0
+}
+Tclass._System.array -> {
+  else -> T@U!val!0
+}
+Tclass._System.array_0 -> {
+  else -> T@U!val!0
+}
+Tclass._System.array? -> {
+  else -> T@U!val!0
+}
+Tclass._System.array?_0 -> {
+  else -> T@U!val!0
+}
+Tclass._System.Tuple2 -> {
+  else -> T@U!val!0
+}
+Tclass._System.Tuple2_0 -> {
+  else -> T@U!val!0
+}
+Tclass._System.Tuple2_1 -> {
+  else -> T@U!val!0
+}
+tickleBool -> {
+  false -> true
+  true -> true
+  else -> true
+}
+TIMap -> {
+  else -> T@U!val!0
+}
+TISet -> {
+  else -> T@U!val!0
+}
+TMap -> {
+  else -> T@U!val!0
+}
+TMultiSet -> {
+  else -> T@U!val!0
+}
+TSeq -> {
+  else -> T@U!val!0
+}
+TSet -> {
+  else -> T@U!val!0
+}
+type -> {
+  false -> T@T!val!2
+  T@U!val!0 -> T@T!val!6
+  T@U!val!1 -> T@T!val!6
+  T@U!val!10 -> T@T!val!7
+  T@U!val!11 -> T@T!val!7
+  T@U!val!12 -> T@T!val!7
+  T@U!val!13 -> T@T!val!7
+  T@U!val!14 -> T@T!val!7
+  T@U!val!15 -> T@T!val!7
+  T@U!val!16 -> T@T!val!7
+  T@U!val!17 -> T@T!val!8
+  T@U!val!18 -> T@T!val!8
+  T@U!val!19 -> T@T!val!8
+  T@U!val!2 -> T@T!val!6
+  T@U!val!20 -> T@T!val!8
+  T@U!val!21 -> T@T!val!8
+  T@U!val!22 -> T@T!val!9
+  T@U!val!23 -> T@T!val!10
+  T@U!val!24 -> T@T!val!7
+  T@U!val!25 -> T@T!val!8
+  T@U!val!26 -> T@T!val!7
+  T@U!val!27 -> T@T!val!7
+  T@U!val!28 -> T@T!val!8
+  T@U!val!29 -> T@T!val!7
+  T@U!val!3 -> T@T!val!6
+  T@U!val!30 -> T@T!val!7
+  T@U!val!31 -> T@T!val!7
+  T@U!val!32 -> T@T!val!7
+  T@U!val!33 -> T@T!val!7
+  T@U!val!34 -> T@T!val!7
+  T@U!val!35 -> T@T!val!7
+  T@U!val!36 -> T@T!val!7
+  T@U!val!37 -> T@T!val!11
+  T@U!val!38 -> T@T!val!7
+  T@U!val!39 -> T@T!val!8
+  T@U!val!4 -> T@T!val!6
+  T@U!val!40 -> T@T!val!11
+  T@U!val!41 -> T@T!val!7
+  T@U!val!42 -> T@T!val!8
+  T@U!val!43 -> T@T!val!8
+  T@U!val!44 -> T@T!val!7
+  T@U!val!45 -> T@T!val!12
+  T@U!val!46 -> T@T!val!12
+  T@U!val!47 -> T@T!val!12
+  T@U!val!48 -> T@T!val!12
+  T@U!val!49 -> T@T!val!12
+  T@U!val!5 -> T@T!val!7
+  T@U!val!50 -> T@T!val!12
+  T@U!val!51 -> T@T!val!12
+  T@U!val!52 -> T@T!val!12
+  T@U!val!53 -> T@T!val!12
+  T@U!val!54 -> T@T!val!12
+  T@U!val!55 -> T@T!val!12
+  T@U!val!56 -> T@T!val!12
+  T@U!val!57 -> T@T!val!6
+  T@U!val!58 -> T@T!val!19
+  T@U!val!59 -> T@T!val!6
+  T@U!val!6 -> T@T!val!7
+  T@U!val!60 -> T@T!val!16
+  T@U!val!61 -> T@T!val!6
+  T@U!val!62 -> T@T!val!6
+  T@U!val!63 -> T@T!val!17
+  T@U!val!64 -> T@T!val!6
+  T@U!val!65 -> T@T!val!19
+  T@U!val!66 -> T@T!val!21
+  T@U!val!7 -> T@T!val!7
+  T@U!val!8 -> T@T!val!7
+  T@U!val!9 -> T@T!val!7
+  else -> T@T!val!7
+}
+TypeTuple -> {
+  else -> T@U!val!0
+}
+TypeTupleCar -> {
+  else -> T@U!val!0
+}
+TypeTupleCdr -> {
+  else -> T@U!val!0
+}
+U_2_bool -> {
+  false -> false
+  else -> false
+}
+U_2_int -> {
+  else -> 0
+}
+U_2_real -> {
+  else -> 0.0
+}
+U_2_regex -> {
+  else -> (str.to.re (""))
+}
+U_2_rmode -> {
+  else -> (roundTowardZero)
+}
+U_2_string -> {
+  else -> ("")
+}
+UOrdering2 -> {
+  else -> false
+}
+UOrdering3 -> {
+  else -> false
+}
+*** STATE <initial>
+  $_Frame -> 
+  $_reverifyPost -> 
+  $Heap -> T@U!val!65
+  $Tick -> 
+  a#0 -> 11
+  b#0 -> 5
+  c#0 -> 
+  defass#c#0 -> 
+*** END_STATE
+*** STATE /workspaces/dafny/string_project/str_recurse.dfy(5,2): initial state
+  $_Frame -> T@U!val!66
+*** END_STATE
+*** END_MODEL
